Functions for options, lists, vectors and mlstrings

basis/basisProgScript.sml
@@ -77,10 +77,232 @@ val _ = register_type ``:order``;
 val _ = register_type ``:'a list``;
 val _ = register_type ``:'a option``;
 
-(* new stuff *)
+(* the parser targets the following for int arith ops -- translated *)
+
+val _ = trans "+" `(+):int->int->int`
+val _ = trans "-" `(-):int->int->int`
+val _ = trans "*" `int_mul`
+val _ = trans "div" `(/):int->int->int`
+val _ = trans "mod" `(%):int->int->int`
+val _ = trans "<" `(<):int->int->bool`
+val _ = trans ">" `(>):int->int->bool`
+val _ = trans "<=" `(<=):int->int->bool`
+val _ = trans ">=" `(>=):int->int->bool`
+val _ = trans "~" `\i. - (i:int)`
+
+
+(* other basics that parser targets -- CF verified *)
+
+val _ = trans "=" `\x1 x2. x1 = x2:'a`
+val _ = trans "not" `\x. ~x:bool`
+val _ = trans "<>" `\x1 x2. x1 <> (x2:'a)`
+
+val _ = append_prog
+  ``[Tdec (mk_binop ":=" Opassign);
+     Tdec (mk_unop "!" Opderef);
+     Tdec (mk_unop "ref" Opref)]``
+
+fun prove_ref_spec op_name =
+  xcf op_name (basis_st ()) \\
+  fs [cf_ref_def, cf_deref_def, cf_assign_def] \\ irule local_elim \\
+  reduce_tac \\ fs [app_ref_def, app_deref_def, app_assign_def] \\
+  xsimpl \\ fs [UNIT_TYPE_def]
+
+val ref_spec = Q.store_thm ("ref_spec",
+  `!xv. app (p:'ffi ffi_proj) ^(fetch_v "op ref" (basis_st())) [xv]
+          emp (POSTv rv. rv ~~> xv)`,
+  prove_ref_spec "op ref");
+
+val deref_spec = Q.store_thm ("deref_spec",
+  `!xv. app (p:'ffi ffi_proj) ^(fetch_v "op !" (basis_st())) [rv]
+          (rv ~~> xv) (POSTv yv. cond (xv = yv) * rv ~~> xv)`,
+  prove_ref_spec "op !");
+
+val assign_spec = Q.store_thm ("assign_spec",
+  `!rv xv yv.
+     app (p:'ffi ffi_proj) ^(fetch_v "op :=" (basis_st())) [rv; yv]
+       (rv ~~> xv) (POSTv v. cond (UNIT_TYPE () v) * rv ~~> yv)`,
+  prove_ref_spec "op :=");
+
+
+(* Word8 module -- translated *)
+
+val _ = ml_prog_update (open_module "Word8");
+
+val _ = append_dec ``Dtabbrev [] "word" (Tapp [] TC_word8)``;
+val _ = trans "fromInt" `n2w:num->word8`
+val _ = trans "toInt" `w2n:word8->num`
+val _ = trans "andb" `word_and:word8->word8->word8`;
+
+val _ = ml_prog_update (close_module NONE);
+
+
+(* Word8Array module -- CF verified *)
+
+val _ = ml_prog_update (open_module "Word8Array");
+
+val _ = append_decs
+   ``[Dtabbrev [] "array" (Tapp [] TC_word8array);
+      Dtabbrev [] "elem" (Tapp [] TC_word8);
+      mk_binop "array" Aw8alloc;
+      mk_binop "sub" Aw8sub;
+      mk_unop "length" Aw8length;
+      Dlet (Pvar "update") (Fun "x" (Fun "y" (Fun "z"
+        (App Aw8update [Var (Short "x"); Var (Short "y"); Var (Short "z")])))) ]``
+
+val _ = ml_prog_update (close_module NONE);
+
+fun prove_array_spec op_name =
+  xcf op_name (basis_st()) \\ TRY xpull \\
+  fs [cf_aw8alloc_def, cf_aw8sub_def, cf_aw8length_def, cf_aw8update_def,
+      cf_aalloc_def, cf_asub_def, cf_alength_def, cf_aupdate_def] \\
+  irule local_elim \\ reduce_tac \\
+  fs [app_aw8alloc_def, app_aw8sub_def, app_aw8length_def, app_aw8update_def,
+      app_aalloc_def, app_asub_def, app_alength_def, app_aupdate_def] \\
+  xsimpl \\ fs [INT_def, NUM_def, WORD_def, w2w_def, UNIT_TYPE_def] \\
+  TRY (simp_tac (arith_ss ++ intSimps.INT_ARITH_ss) [])
+
+val w8array_alloc_spec = Q.store_thm ("w8array_alloc_spec",
+  `!n nv w wv.
+     NUM n nv /\ WORD w wv ==>
+     app (p:'ffi ffi_proj) ^(fetch_v "Word8Array.array" (basis_st())) [nv; wv]
+       emp (POSTv v. W8ARRAY v (REPLICATE n w))`,
+  prove_array_spec "Word8Array.array");
+
+val w8array_sub_spec = Q.store_thm ("w8array_sub_spec",
+  `!a av n nv.
+     NUM n nv /\ n < LENGTH a ==>
+     app (p:'ffi ffi_proj) ^(fetch_v "Word8Array.sub" (basis_st())) [av; nv]
+       (W8ARRAY av a) (POSTv v. cond (WORD (EL n a) v) * W8ARRAY av a)`,
+  prove_array_spec "Word8Array.sub");
+
+val w8array_length_spec = Q.store_thm ("w8array_length_spec",
+  `!a av.
+     app (p:'ffi ffi_proj) ^(fetch_v "Word8Array.length" (basis_st())) [av]
+       (W8ARRAY av a) (POSTv v. cond (NUM (LENGTH a) v) * W8ARRAY av a)`,
+  prove_array_spec "Word8Array.length");
+
+val w8array_update_spec = Q.store_thm ("w8array_update_spec",
+  `!a av n nv w wv.
+     NUM n nv /\ n < LENGTH a /\ WORD w wv ==>
+     app (p:'ffi ffi_proj) ^(fetch_v "Word8Array.update" (basis_st()))
+       [av; nv; wv]
+       (W8ARRAY av a)
+       (POSTv v. cond (UNIT_TYPE () v) * W8ARRAY av (LUPDATE w n a))`,
+  prove_array_spec "Word8Array.update");
+
+
+
+(* Array module -- CF verified *)
+
+val _ = ml_prog_update (open_module "Array");
+
+val _ = append_decs
+   ``[Dtabbrev ["'a"] "array" (Tapp [Tvar "'a"] TC_array);
+      mk_binop "array" Aalloc;
+      mk_binop "sub" Asub;
+      mk_unop "length" Alength;
+      Dlet (Pvar "update")
+       (Fun "x" (Fun "y" (Fun "z"
+         (App Aupdate [Var (Short "x"); Var (Short "y"); Var (Short "z")])))) ]``
+
+val _ = ml_prog_update (close_module NONE);
+
+val array_alloc_spec = Q.store_thm ("array_alloc_spec",
+  `!n nv v.
+     NUM n nv ==>
+     app (p:'ffi ffi_proj) ^(fetch_v "Array.array" (basis_st())) [nv; v]
+       emp (POSTv av. ARRAY av (REPLICATE n v))`,
+  prove_array_spec "Array.array");
+
+val array_sub_spec = Q.store_thm ("array_sub_spec",
+  `!a av n nv.
+     NUM n nv /\ n < LENGTH a ==>
+     app (p:'ffi ffi_proj) ^(fetch_v "Array.sub" (basis_st())) [av; nv]
+       (ARRAY av a) (POSTv v. cond (v = EL n a) * ARRAY av a)`,
+  prove_array_spec "Array.sub");
+
+val array_length_spec = Q.store_thm ("array_length_spec",
+  `!a av.
+     app (p:'ffi ffi_proj) ^(fetch_v "Array.length" (basis_st())) [av]
+       (ARRAY av a)
+       (POSTv v. cond (NUM (LENGTH a) v) * ARRAY av a)`,
+  prove_array_spec "Array.length");
+
+val array_update_spec = Q.store_thm ("array_update_spec",
+  `!a av n nv v.
+     NUM n nv /\ n < LENGTH a ==>
+     app (p:'ffi ffi_proj) ^(fetch_v "Array.update" (basis_st()))
+       [av; nv; v]
+       (ARRAY av a)
+       (POSTv uv. cond (UNIT_TYPE () uv) * ARRAY av (LUPDATE v n a))`,
+  prove_array_spec "Array.update");
+
+(*new stuff*)
 (*################################################################################*)
 
+(* Option module -- Translated *)
+
+val _ = ml_prog_update (open_module "Option");
+
+val _ = append_dec ``Dtabbrev ["'a"] "option" (Tapp [Tvar "'a"] (TC_name (Short "option")))``;
+
+val result = translate IS_SOME_DEF;
+
+val getOpt_def = Define`
+  getOpt opt a = case opt of
+    (SOME v) => v
+    | NONE => a`;
+
+val result = translate getOpt_def;
+
+val result = translate IS_SOME_DEF;  
+
+
+(*precondition/option exception if it is not in the form (SOME x) *)
+val result = next_ml_names := ["valOf_def"];
+val result = translate THE_DEF;
+
+val filter_def  = Define`
+  filter f a = if f a then SOME(a) else NONE`;
+val result = translate filter_def;
+
+val result = next_ml_names := ["join_def"];
+val result = translate OPTION_JOIN_DEF; 
+
+(*app still missing *)
+
+val result = next_ml_names := ["map_def"];
+val result = translate OPTION_MAP_DEF;
+
+val mapPartial_def = Define`
+  mapPartial f opt = OPTION_BIND opt f`;
+val result = translate (OPTION_BIND_def |> REWRITE_RULE[GSYM mapPartial_def]);
+
+(*val compose_def = Define`
+  compose f g a = ((OPTION_MAP f) o g) a`;
+val result = translate (OPTION_MAP_DEF |> REWRITE_RULE[GSYM compose_def]);
+*)
+
+val compose_def = Define`
+  compose f g a = case g a of 
+    (SOME v) => SOME(f v)
+    | NONE => NONE`;
+val result = translate compose_def;
+
+val composePartial_def = Define`
+  composePartial f g a = case g a of
+    (SOME v) => f v
+    | NONE => NONE`;
+val result = translate composePartial_def;
+
+val _ = ml_prog_update (close_module NONE);
+
+(*################################################################################*)
+(*End new stuff *)
+
 (* List module -- Translated *)
+
 
 (* TODO: move this module into its own theory and check the translator to allow
 names that save_thm can't handle, see if translation is being module specific
@@ -107,21 +329,21 @@ val result = translate APPEND;
 (*--------------------------------------------------------------------------------*)
 
 show_assums := true;
-(*This has a precondition and I don't know what is wanted with pattern matching,
-  list empty exception*)
+(*This has a precondition, list empty exception*)
 val result = translate HD;
-val hd_side_def = definition"hd_side_def"
 
 (*--------------------------------------------------------------------------------*)
 
-(*This has a precondition and I don't know what is wanted with pattern matching, 
-  list empty exception*)
+(*This has a precondition, list empty exception*)
 val result = translate TL;
 
 (*--------------------------------------------------------------------------------*)
 
 (*Pre-conditions needs to raise an exception with the list is empty *)
+
 val result = translate LAST_DEF;
+val last_side_def = theorem"last_side_def"
+
 
 (*--------------------------------------------------------------------------------*)
 
@@ -135,38 +357,27 @@ val result = translate getItem_def;
 (*--------------------------------------------------------------------------------*)
 
 val nth_def = Define`
-  nth (l, i) = EL i l`;
+  nth l i = EL i l`;
+val result = translate (EL |> REWRITE_RULE[GSYM nth_def]);
 (*EL has a precondition because TL and HD have preconditions, subscript exception *)
-val result = translate EL;
-val result = translate nth_def;
 
 (*--------------------------------------------------------------------------------*)
 
 (*subscript exception *)
 val take_def = Define`
-  take (l, i) = TAKE i l`;
-(*see if this is correct *)
-val result = next_ml_names := ["TAKE_HOL"];
-val result = translate TAKE_def;
-val result = translate take_def;
+  take l i = TAKE i l`;
+val result = translate (TAKE_def |> REWRITE_RULE[GSYM take_def]);
 
 (*--------------------------------------------------------------------------------*)
 
 val drop_def = Define`
-  drop (l, i) = DROP i l`;
-val result = next_ml_names := ["DROP_HOL"];
-val result = translate DROP_def;
-val result = translate drop_def;
+  drop l i = DROP i l`;
+val result = translate (DROP_def |> REWRITE_RULE[GSYM drop_def]);
 
 (*--------------------------------------------------------------------------------*)
 
-(*
-val rev_def = Define`
-  rev l = REVERSE l`;
-*)
 val result = next_ml_names := ["rev_def"];
 val result = translate REVERSE_DEF;
-(* val result = translate rev_def; *)
 
 (*--------------------------------------------------------------------------------*)
 
@@ -175,14 +386,11 @@ val result = translate FLAT;
 
 (*--------------------------------------------------------------------------------*)
 
-val revAppend_def = Define`
-  revAppend (l1, l2) = REV l1 l2`;
 val result = translate REV_DEF;
-val result = translate revAppend_def;
 
 (*--------------------------------------------------------------------------------*)
 
-(*What do we do with app?? *)
+(*List.app needs to be decided upon *)
 
 (*--------------------------------------------------------------------------------*)
 
@@ -193,33 +401,77 @@ val result = translate MAP;
 val mapPartial_def = Define`
   mapPartial f l = case l of
     [] => []
-    | (h::t) => if f h = NONE then h::(mapPartial f t)
-      else mapPartial f t`;
+    | (h::t) => case (f h) of     
+      NONE => mapPartial f t
+      | (SOME x) => x::(mapPartial f t)`;
+
 val result = translate mapPartial_def;   
+
+val mapPartial_thm = Q.store_thm (
+  "mapPartial_thm",
+  `!f l. mapPartial f l = MAP THE (FILTER IS_SOME (MAP f l))`,
+  Induct_on `l` THEN1
+  rw [mapPartial_def] \\
+  rw [mapPartial_def] \\
+  Cases_on `f h` THEN1
+    fs [IS_SOME_DEF]\\
+    rw [THE_DEF] \\
+  Cases_on `f h` THEN1
+    rw [] \\
+    fs [IS_SOME_DEF]
+)
+
+
 
 (*--------------------------------------------------------------------------------*)
 
+
+(*note that I didn't just translate find because it uses a method which stores indexes
+ and values and then has to peel the value from a pair *)
 val find_def = Define`
   find f l = case l of
     [] => NONE
-    | (h::t) => if f h = NONE then find f t
-      else h`;
+    | (h::t) => if f h then SOME(h)
+      else find f t`;
 val result = translate find_def;
 
+
+val index_find_thm = Q.prove (
+  `!x y. OPTION_MAP SND (INDEX_FIND x f l) = OPTION_MAP SND (INDEX_FIND y f l)`,
+  Induct_on `l` THEN1
+  rw [INDEX_FIND_def] \\
+  Cases_on `f h` \\
+  EVAL_TAC \\
+  rw [] \\
+  EVAL_TAC \\
+  rw [] 
+);
+
+
+"find_thm",
+  `!f l. find f l = FIND f l`,
+  Induct_on `l` \\
+  rw [find_def, FIND_def, INDEX_FIND_def] \\
+  rw [find_def, FIND_def] \\
+  rw [INDEX_FIND_def] \\
+  EVAL_TAC \\
+  rw [index_find_thm]
+)
+
+
+
+
+
 (*--------------------------------------------------------------------------------*)
 
-val filter_def = Define`
-  filter f l = case l of
-    [] => []
-    | (h::t) => if f h then h::(filter f t)
-      else filter f t`;
-val result = translate filter_def; 
+val result = translate FILTER;
 
 (*--------------------------------------------------------------------------------*)
 
+(*check if pos and neg should be curried *)
 val partition_aux_def = Define`
   partition_aux f l (pos, neg) = case l of
-    [] => (pos, neg)
+    [] => (REVERSE pos, REVERSE neg)
     | (h::t) => if f h then partition_aux f t ((h::pos), neg)
       else partition_aux f t (pos, (h::neg))`;
 
@@ -228,6 +480,7 @@ val partition_def = Define`
 
 val result = translate partition_aux_def;
 val result = translate partition_def;
+
 
 (*--------------------------------------------------------------------------------*)
 
@@ -248,27 +501,69 @@ val result = translate EVERY_DEF;
 
 (*--------------------------------------------------------------------------------*)
 
+(* raise exception for n < 0 *)
 val tabulate_def = Define`
-  tabulate (n, f) = GENLIST f n`;
+  tabulate n f = GENLIST f n`;
+val result = translate SNOC;
 val result = translate GENLIST_AUX;
 val result = translate GENLIST_GENLIST_AUX;
-val result = translate tabulate_def;
+val result = translate (GENLIST |> REWRITE_RULE[GSYM tabulate_def]);
 
 (*--------------------------------------------------------------------------------*)
 
-(* TODO: Check the functionality of this function *)
+(*This function has been curried to be different to SML *)
 val collate_def = Define`
-  collate f (l1, l2) = case l1 of
+  collate f l1 l2 = case l1 of
     [] => (case l2 of
       [] => EQUAL
       | (h2::t2) => GREATER)
     | (h1::t1) => (case l2 of
       [] => LESS
-      | (h2::t2) => if f h1 h2 = EQUAL then collate f (t1, t2)
+      | (h2::t2) => if f h1 h2 = EQUAL then collate f t1 t2
         else f h1 h2)`;
 val result = translate collate_def;
 
+
 (*--------------------------------------------------------------------------------*)
+val zip_def = Define`
+  zip l1 l2 = 
+    case l1 of
+      (h1::t1) => (case l2 of
+        [] => []
+        | (h2::t2) => (h1, h2)::(zip t1 t2))
+      | [] => []`; 
+
+val result = translate zip_def;
+
+(*--------------------------------------------------------------------------------*)
+
+val butLast_def = Define`
+  butLast  l = case l of
+      [] => [] (*this is to stop exceptions*)
+      | (h::t) => 
+        if t = [] 
+          then []
+        else h::(butLast t)`;
+
+val result = translate butLast_def;
+
+(*--------------------------------------------------------------------------------*)
+
+(*Haskell Functions*)
+val scanl_def = Define`
+  scanl f q l = q::(case l of
+      [] => []
+      | (h::t) => scanl f (f q h) t)`;
+
+val result = translate scanl_def;
+
+(*--------------------------------------------------------------------------------*)
+
+(*this is a reasonably poor implementation *)
+val scanr_def = Define`
+  scanr_def f q l = REVERSE (scanl f q (REVERSE l))`;
+
+val result = translate scanr_def;
 val _ = ml_prog_update (close_module NONE);
 
 (* end new stuff *)
@@ -399,16 +694,9 @@ val concat_def = Define`
   concat l = Vector (FLAT (concat_aux l 0))`;
 *)
 
-(*TODO prove concat works *)
 val concat_def = Define`
   concat l = Vector (FLAT (MAP toList l))`;
 
-(* 
-val result = translate APPEND;
-val next_ml_names = ["concat"];
-val result = translate FLAT; 
-val result = translate MAP;
-*)
 val result = translate concat_def;
 
 
@@ -434,6 +722,7 @@ val result = translate concat_def;
   val appi_aux_def = xDefine "app_aux"`
     appi_aux f vec n = if length vec <= n then vec
       else appi_aux f (update vec n (f n (sub vec n))) (n + 1)`
+
   (
     wf_rel_tac `measure (\(f, vec, n). length(vec) - n)` \\
     Cases_on `vec` \\
@@ -455,188 +744,195 @@ val map_def = Define`
 val mapi_def = Define`
   mapi vec f = tabulate (length vec) (\n. f n (sub vec n))`; 
 
-val map_proof_def = Define`
-  map_proof vec f = fromList (MAP f (toList vec))`;
-
-(*TODO find a way to implement mapi using the list MAP function *)
+val map_thm = Q.store_thm (
+  "map_thm",
+  `!vec f. map vec f = fromList (MAP f (toList vec))`,
+  Cases \\
+  rw [map_def, toList_thm, length_def, sub_def, tabulate_def, fromList_def, 
+    GENLIST_EL_MAP]
+);  
 
 show_assums := true;
 
-(* map is already defined in the translator for strings check if this still works *)
-(*TODO fix map side condition if need be*)
 val result = translate map_def;
 val map_1_side_def = definition"map_1_side_def";
 val result = translate mapi_def;
 
+(*--------------------------------------------------------------------------------*)
+
+val foldli_aux_def = tDefine "foldli_aux"`
+  foldli_aux f e vec (max: num) n = 
+    if max <= n 
+      then e
+    else foldli_aux f (f n e (sub vec n)) vec max (n + 1)`
+(wf_rel_tac `measure (\(f, e, vec, max, n). max - n)`);
+
+val foldli_def = Define`
+  foldli f e vec = foldli_aux f e vec (length vec) 0`; 
+
+val result = translate foldli_aux_def;
+val result = translate foldli_def;
+
+
+val foldl_aux_def = tDefine "foldl_aux"`
+  foldl_aux f e vec (max: num) n = 
+    if max <= n
+      then e
+    else foldl_aux f (f e (sub vec n)) vec max (n + 1)`
+(wf_rel_tac `measure (\(f, e, vec, max, n). max - n)`);
+
+val foldl_def = Define`
+  foldl f e vec = foldl_aux f e vec (length vec) 0`;
+
+val result = translate foldl_aux_def;
+val result = translate foldl_def;
+
+
+val foldl_thm = Q.store_thm (
+  "foldl_thm",
+  `!f e vec. foldl f e vec = fromList (FOLDL f e (toList vec))`,
+  Cases \\
+  rw [map_def, toList_thm, length_def, sub_def, tabulate_def, fromList_def, 
+    GENLIST_EL_MAP]
+); 
+ 
+`!f e vec. foldl f e vec = FOLDL f e (toList vec)`
+Cases \\
+rw [toList_def, toList_aux_thm]
+Cases
+
+
+
 
 (*--------------------------------------------------------------------------------*)
+
+val foldri_aux_def = tDefine "foldri_aux"`
+  foldri_aux f e vec (n: num) = 
+    if n = 0 
+      then f e 0
+    else foldri_aux f (f n e (sub vec n)) vec (n - 1)`
+(wf_rel_tac `measure (\(f, e, vec, n). n)`);
+
+val foldri_def = Define`
+  foldri f e vec = foldri_aux f e vec ((length vec) - 1)`; 
+
+val result = translate foldri_aux_def;
+val result = translate foldri_def;
+
+
+val foldr_aux_def = tDefine "foldr_aux"`
+  foldr_aux f e vec (n: num) = 
+    if n = 0
+      then e
+    else foldr_aux f (f e (sub vec n)) vec (n - 1)`
+(wf_rel_tac `measure (\(f, e, vec, n). n)`);
+
+val foldr_def = Define`
+  foldl f e vec = foldr_aux f e vec ((length vec) - 1)`;
+
+val result = translate foldr_aux_def;
+val result = translate foldr_def;
+
+
+(*--------------------------------------------------------------------------------*)
+
+val findi_aux_def = tDefine "findi_aux"`
+  findi_aux f vec max n =
+    if max <= n 
+      then NONE
+    else if f n (sub vec n)
+      then SOME(sub vec n)
+    else findi_aux f vec max (n + 1)`
+(wf_rel_tac `measure (\(f, vec, max, n). max - n)`);
+
+val findi_def = Define `
+  findi f vec = findi_aux f vec (length vec) 0`;
+
+val result = translate findi_aux_def;
+val result = translate findi_def;
+
+
+val find_aux_def = tDefine "find_aux"`
+  find_aux f vec max n =
+    if max <= n 
+      then NONE
+    else if f (sub vec n)
+      then SOME(sub vec n)
+    else find_aux f vec max (n + 1)`
+(wf_rel_tac `measure (\(f, vec, max, n). max - n)`);
+
+val find_def = Define `
+  find f vec = find_aux f vec (length vec) 0`;
+
+val result = translate find_aux_def;
+val result = translate find_def;
+
+
+(*--------------------------------------------------------------------------------*)
+
+val exists_aux_def = tDefine "exists_aux"`
+  exists_aux f vec max n =
+    if max <= n
+      then F
+    else if f (sub vec n)
+      then T
+    else exists_aux f vec max (n + 1)`
+(wf_rel_tac `measure (\(f, vec, max, n). max - n)`);
+
+val exists_def = Define`
+  exists f vec = exists_aux f vec (length vec) 0`;
+
+val result = translate exists_aux_def;
+val result = translate exists_def;
+
+(*--------------------------------------------------------------------------------*)
+
+val all_aux_def = tDefine "all_aux"`
+  all_aux f vec max n =
+    if max <= n
+      then T
+    else if f (sub vec n)
+      then all_aux f vec max (n + 1)
+    else F`
+(wf_rel_tac `measure (\(f, vec, max, n). max - n)`);
+
+val all_def = Define`
+  all f vec = all_aux f vec (length vec) 0`;
+
+val result = translate all_aux_def;
+val result = translate all_def;
+
+
+(*--------------------------------------------------------------------------------*)
+
+val collate_aux_def = tDefine "collate_aux"`
+  collate_aux f vec1 vec2 max ord n =
+    if max <= n
+      then ord
+    else if f (sub vec1 n) (sub vec2 n) = EQUAL
+      then collate_aux f vec1 vec2 max ord (n + 1)
+    else
+      f (sub vec1 n) (sub vec2 n)`
+(wf_rel_tac `measure (\(f, vec1, vec2, max, ord, n). max - n)`);
+
+val collate_def = Define`
+  collate f vec1 vec2 =
+  if (length vec1) < (length vec2)
+    then collate_aux f vec1 vec2 (length vec1) GREATER 0
+  else if (length vec2) < (length vec1)
+    then collate_aux f vec1 vec2 (length vec2) LESS 0
+  else collate_aux f vec1 vec2 (length vec2) EQUAL 0`;
+
+val result = translate collate_aux_def;
+val result = translate collate_def;
+
 
 val _ = ml_prog_update (close_module NONE);
 
 (*################################################################################*)
 (*end new stuff*)
 
-(* the parser targets the following for int arith ops -- translated *)
 
-val _ = trans "+" `(+):int->int->int`
-val _ = trans "-" `(-):int->int->int`
-val _ = trans "*" `int_mul`
-val _ = trans "div" `(/):int->int->int`
-val _ = trans "mod" `(%):int->int->int`
-val _ = trans "<" `(<):int->int->bool`
-val _ = trans ">" `(>):int->int->bool`
-val _ = trans "<=" `(<=):int->int->bool`
-val _ = trans ">=" `(>=):int->int->bool`
-val _ = trans "~" `\i. - (i:int)`
-
-
-(* other basics that parser targets -- CF verified *)
-
-val _ = trans "=" `\x1 x2. x1 = x2:'a`
-val _ = trans "not" `\x. ~x:bool`
-val _ = trans "<>" `\x1 x2. x1 <> (x2:'a)`
-
-val _ = append_prog
-  ``[Tdec (mk_binop ":=" Opassign);
-     Tdec (mk_unop "!" Opderef);
-     Tdec (mk_unop "ref" Opref)]``
-
-fun prove_ref_spec op_name =
-  xcf op_name (basis_st ()) \\
-  fs [cf_ref_def, cf_deref_def, cf_assign_def] \\ irule local_elim \\
-  reduce_tac \\ fs [app_ref_def, app_deref_def, app_assign_def] \\
-  xsimpl \\ fs [UNIT_TYPE_def]
-
-val ref_spec = Q.store_thm ("ref_spec",
-  `!xv. app (p:'ffi ffi_proj) ^(fetch_v "op ref" (basis_st())) [xv]
-          emp (POSTv rv. rv ~~> xv)`,
-  prove_ref_spec "op ref");
-
-val deref_spec = Q.store_thm ("deref_spec",
-  `!xv. app (p:'ffi ffi_proj) ^(fetch_v "op !" (basis_st())) [rv]
-          (rv ~~> xv) (POSTv yv. cond (xv = yv) * rv ~~> xv)`,
-  prove_ref_spec "op !");
-
-val assign_spec = Q.store_thm ("assign_spec",
-  `!rv xv yv.
-     app (p:'ffi ffi_proj) ^(fetch_v "op :=" (basis_st())) [rv; yv]
-       (rv ~~> xv) (POSTv v. cond (UNIT_TYPE () v) * rv ~~> yv)`,
-  prove_ref_spec "op :=");
-
-
-(* Word8 module -- translated *)
-
-val _ = ml_prog_update (open_module "Word8");
-
-val _ = append_dec ``Dtabbrev [] "word" (Tapp [] TC_word8)``;
-val _ = trans "fromInt" `n2w:num->word8`
-val _ = trans "toInt" `w2n:word8->num`
-val _ = trans "andb" `word_and:word8->word8->word8`;
-
-val _ = ml_prog_update (close_module NONE);
-
-
-(* Word8Array module -- CF verified *)
-
-val _ = ml_prog_update (open_module "Word8Array");
-
-val _ = append_decs
-   ``[Dtabbrev [] "array" (Tapp [] TC_word8array);
-      Dtabbrev [] "elem" (Tapp [] TC_word8);
-      mk_binop "array" Aw8alloc;
-      mk_binop "sub" Aw8sub;
-      mk_unop "length" Aw8length;
-      Dlet (Pvar "update") (Fun "x" (Fun "y" (Fun "z"
-        (App Aw8update [Var (Short "x"); Var (Short "y"); Var (Short "z")])))) ]``
-
-val _ = ml_prog_update (close_module NONE);
-
-fun prove_array_spec op_name =
-  xcf op_name (basis_st()) \\ TRY xpull \\
-  fs [cf_aw8alloc_def, cf_aw8sub_def, cf_aw8length_def, cf_aw8update_def,
-      cf_aalloc_def, cf_asub_def, cf_alength_def, cf_aupdate_def] \\
-  irule local_elim \\ reduce_tac \\
-  fs [app_aw8alloc_def, app_aw8sub_def, app_aw8length_def, app_aw8update_def,
-      app_aalloc_def, app_asub_def, app_alength_def, app_aupdate_def] \\
-  xsimpl \\ fs [INT_def, NUM_def, WORD_def, w2w_def, UNIT_TYPE_def] \\
-  TRY (simp_tac (arith_ss ++ intSimps.INT_ARITH_ss) [])
-
-val w8array_alloc_spec = Q.store_thm ("w8array_alloc_spec",
-  `!n nv w wv.
-     NUM n nv /\ WORD w wv ==>
-     app (p:'ffi ffi_proj) ^(fetch_v "Word8Array.array" (basis_st())) [nv; wv]
-       emp (POSTv v. W8ARRAY v (REPLICATE n w))`,
-  prove_array_spec "Word8Array.array");
-
-val w8array_sub_spec = Q.store_thm ("w8array_sub_spec",
-  `!a av n nv.
-     NUM n nv /\ n < LENGTH a ==>
-     app (p:'ffi ffi_proj) ^(fetch_v "Word8Array.sub" (basis_st())) [av; nv]
-       (W8ARRAY av a) (POSTv v. cond (WORD (EL n a) v) * W8ARRAY av a)`,
-  prove_array_spec "Word8Array.sub");
-
-val w8array_length_spec = Q.store_thm ("w8array_length_spec",
-  `!a av.
-     app (p:'ffi ffi_proj) ^(fetch_v "Word8Array.length" (basis_st())) [av]
-       (W8ARRAY av a) (POSTv v. cond (NUM (LENGTH a) v) * W8ARRAY av a)`,
-  prove_array_spec "Word8Array.length");
-
-val w8array_update_spec = Q.store_thm ("w8array_update_spec",
-  `!a av n nv w wv.
-     NUM n nv /\ n < LENGTH a /\ WORD w wv ==>
-     app (p:'ffi ffi_proj) ^(fetch_v "Word8Array.update" (basis_st()))
-       [av; nv; wv]
-       (W8ARRAY av a)
-       (POSTv v. cond (UNIT_TYPE () v) * W8ARRAY av (LUPDATE w n a))`,
-  prove_array_spec "Word8Array.update");
-
-val _ = ml_prog_update (close_module NONE);
-
-
-(* Array module -- CF verified *)
-
-val _ = ml_prog_update (open_module "Array");
-
-val _ = append_decs
-   ``[Dtabbrev ["'a"] "array" (Tapp [Tvar "'a"] TC_array);
-      mk_binop "array" Aalloc;
-      mk_binop "sub" Asub;
-      mk_unop "length" Alength;
-      Dlet (Pvar "update")
-       (Fun "x" (Fun "y" (Fun "z"
-         (App Aupdate [Var (Short "x"); Var (Short "y"); Var (Short "z")])))) ]``
-
-val _ = ml_prog_update (close_module NONE);
-
-val array_alloc_spec = Q.store_thm ("array_alloc_spec",
-  `!n nv v.
-     NUM n nv ==>
-     app (p:'ffi ffi_proj) ^(fetch_v "Array.array" (basis_st())) [nv; v]
-       emp (POSTv av. ARRAY av (REPLICATE n v))`,
-  prove_array_spec "Array.array");
-
-val array_sub_spec = Q.store_thm ("array_sub_spec",
-  `!a av n nv.
-     NUM n nv /\ n < LENGTH a ==>
-     app (p:'ffi ffi_proj) ^(fetch_v "Array.sub" (basis_st())) [av; nv]
-       (ARRAY av a) (POSTv v. cond (v = EL n a) * ARRAY av a)`,
-  prove_array_spec "Array.sub");
-
-val array_length_spec = Q.store_thm ("array_length_spec",
-  `!a av.
-     app (p:'ffi ffi_proj) ^(fetch_v "Array.length" (basis_st())) [av]
-       (ARRAY av a)
-       (POSTv v. cond (NUM (LENGTH a) v) * ARRAY av a)`,
-  prove_array_spec "Array.length");
-
-val array_update_spec = Q.store_thm ("array_update_spec",
-  `!a av n nv v.
-     NUM n nv /\ n < LENGTH a ==>
-     app (p:'ffi ffi_proj) ^(fetch_v "Array.update" (basis_st()))
-       [av; nv; v]
-       (ARRAY av a)
-       (POSTv uv. cond (UNIT_TYPE () uv) * ARRAY av (LUPDATE v n a))`,
-  prove_array_spec "Array.update");
 
 
 (* Char module -- translated *)
@@ -654,6 +950,7 @@ val _ = trans ">=" `string$char_ge`
 val _ = ml_prog_update (close_module NONE);
 
 
+(*################################################################################*)
 (* String module -- translated *)
 
 val _ = ml_prog_update (open_module "String");
@@ -663,7 +960,294 @@ val _ = trans "explode" `explode`
 val _ = trans "implode" `implode`
 val _ = trans "size" `strlen`
 
+(*new stuff*)
+(*--------------------------------------------------------------------------------*)
+val sub_def = Define`
+  sub s n =  EL n (explode s)`;
+
+(*EL is not translated in list - its translation is moved to nth *)
+val result = translate EL;
+val result = translate sub_def;
+
+(*--------------------------------------------------------------------------------*)
+
+val extract_aux_def = tDefine "extract_aux"`
+    extract_aux s n max =
+    if max <= n
+      then []
+    else (sub s n)::(extract_aux s (n + 1) max)`
+(wf_rel_tac `measure (\(s, n, max). max - n)`)
+
+(*should raise subscript exceptions, THE means there is an option dependency*)
+val extract_def = Define`
+  extract s i opt = case opt of
+    (SOME x) => implode (extract_aux s i (THE opt))
+    | NONE => implode (extract_aux s i (strlen s))`;
+
+val substring_def = Define`
+  substring s i j = implode (extract_aux s i j)`;
+
+(*extract_aux has a pre-condition because sub has a precondition *)
+val result = translate extract_aux_def;
+val result = translate extract_def;
+val result = translate substring_def;
+
+(*--------------------------------------------------------------------------------*)
+
+
+val strcat_def = Define`
+  strcat s1 s2 = implode((explode s1) ++ (explode s2))`
+(*This infix code is from the previous stringml stuff *)
+val _ = Parse.add_infix("^",480,Parse.LEFT)
+val _ = Parse.overload_on("^",``λx y. strcat x y``)
+
+
+val result = translate strcat_def;
+
+(*--------------------------------------------------------------------------------*)
+
+(*at the moment the only way of putting strings together is turning them to lists *)
+val stringListToChars_def = Define`
+  stringListToChars l = case l of 
+    [] => []
+    | ([]::t) => stringListToChars t
+    | ((hh::ht)::t) => hh::stringListToChars(ht::t)`;
+
+fun stringListToChars l = case l of
+    [] => []
+    | ([]::t) => stringListToChars t
+    | ((hh::ht)::t) => hh::stringListToChars(ht::t);
+
+
+(*a more memory efficient implementation *)
+val concat_def = Define`
+  concat l = implode (stringListToChars l)` ;
+(*
+val concat_def = Define`
+  concat l = implode (FLAT (MAP explode l))`;
+*)
+val result = translate stringListToChars_def;
+val result = translate concat_def;
+ 
+(*--------------------------------------------------------------------------------*)
+
+(*NEED TO PROVE TERMINATION*)
+(*may be a bit complex to attempt to save memory (passing around a lot)*)
+val concatWith_aux_def = Define`
+  concatWith_aux l s ss bool =  
+  if bool then
+    case l of
+      [] => []
+      | []::[] => []
+      | ([]::t) => concatWith_aux t s s F
+      | ((hh::ht)::t) => hh::(concatWith_aux (ht::t) s ss T)
+  else 
+    case ss of
+      [] => concatWith_aux l s ss T
+      | (h::t) => h::(concatWith_aux l s t F) `;
+(wf_rel_tac `measure (\(l, s, ss, bool). (LENGTH l) + (LENGTH ss) + (LENGTH (EL 0 l))`)
+
+
+fun concatWith_aux l s ss bool =  
+  if bool then
+    case l of
+         [] => []
+      |  []::[] => []
+      | ([]::t) => concatWith_aux t s ss false
+      | ((hh::ht)::t) => hh::(concatWith_aux (ht::t) s ss true)
+  else 
+    case ss of
+      [] => concatWith_aux l s s true
+      | (h::t) => h::(concatWith_aux l s t false);
+
+val concatWith_def = Define`
+    concatWith s l = implode (concatWith_aux l s s T)`; 
+
+
+(*--------------------------------------------------------------------------------*)
+
+val str_def = Define`
+  str (c: char) = [c]`; 
+
+translate str_def;
+
+(*--------------------------------------------------------------------------------*)
+
+(*not transferred accross because explode is currently a primitive *)
+val explode_aux_def = tDefine "explode_aux"`
+  explode_aux s max n = 
+    if max <= n then []
+    else (sub s n)::(explode_aux s max (n + 1))`
+(wf_rel_tac `measure (\(s, max, n). max - n)`);
+
+val explode_def = Define`
+  explode s = explode_aux s (strlen s) 0`;
+
+translate explode_aux_def;
+translate explode_def;
+
+
+(*--------------------------------------------------------------------------------*)
+
+(*NOTE: MAP for strings is like APP for other types *)
+  
+val translate_aux_def = tDefine "translate_aux"`
+  translate_aux f s max n = 
+    if max <= n then []
+    else f (sub s n)::(translate_aux f s max (n + 1))`
+(wf_rel_tac `measure (\(f, s, max, n). max - n)`);
+
+
+val translate_def = Define`
+  translate f s = implode (translate_aux f s (strlen s) 0)`;
+
+(*these have pre-conditions because sub has a precondition *)
+val result = translate translate_aux_def;
+val result = translate translate_def;
+
+(*--------------------------------------------------------------------------------*)
+
+
+(*Check the functionality *)
+val tokens_aux_def = tDefine "tokens_aux"`
+  tokens_aux f s ss max n = 
+  if max <= n 
+    then []
+  else if (f (sub s n) /\ ~(ss = []))
+    then ss::(tokens_aux f s [] max (n + 1))
+  else if f (sub s n) 
+    then tokens_aux f s ss max (n + 1)
+  else tokens_aux f s ((sub s n)::ss) max (n + 1)`
+(wf_rel_tac `measure (\(f, s, ss, max, n). max - n)`);
+
+val tokens_def = Define `
+  tokens f s = tokens_aux f s [] (strlen s) 0`;
+
+fun tokens_aux (f : char -> bool) s ss max n = 
+  if max <= n 
+    then []
+  else if (f (String.sub s n)) andalso not(ss = [])
+    then ss::(tokens_aux f s [] max (n + 1))
+  else if f (String.sub s n) 
+    then tokens_aux f s ss max (n + 1)
+  else tokens_aux f s ((String.sub s n)::ss) max (n + 1)
+
+
+
+(*these have pre-conditions because sub has a precondition *)
+val result = translate tokens_aux_def;
+val result = translate tokens_def;
+
+(*--------------------------------------------------------------------------------*)
+
+val fields_aux_def = tDefine "fields_aux"`
+  fields_aux f s ss max n = 
+  if max <= n 
+    then []
+  else if f (sub s n)
+    then ss::(fields_aux f s [] max (n + 1))
+  else fields_aux f s ((sub s n)::ss) max (n + 1)`
+(wf_rel_tac `measure (\(f, s, ss, max, n). max - n)`);
+
+val fields_def = Define`
+  fields f s = fields_aux f s [] (strlen s) 0`;
+
+(*these have pre-conditions because sub has a precondition *)
+val result = translate fields_aux_def;
+val result = translate tokens_def;
+
+
+(*--------------------------------------------------------------------------------*)
+
+(*this could be one less iteration if the check is for n + 1 *)
+val isStringThere_aux_def = tDefine "isPrefix_aux"`
+  isStringThere_aux s1 s2 max n = 
+  if max <= n 
+    then T
+  else if (sub s1 n) = (sub s2 n)
+    then isStringThere_aux s1 s2 max (n + 1)
+  else F`
+(wf_rel_tac `measure (\(s1, s2, max, n). max - n)`);
+
+val isPrefix_def = Define`
+  isPrefix s1 s2 = isStringThere_aux s1 s2 (strlen s1) 0`;
+
+val isSuffix_def = Define`
+  isSuffix s1 s2 = isStringThere_aux s1 s2 (strlen s2) ((strlen s2) - (strlen s1))`;
+
+val isSubstring_aux_def = tDefine "isSubstring_aux"`
+  isSubstring_aux s1 s2 len1 max n = 
+    if max <= n
+      then F
+    else if isStringThere_aux s1 s2 (n + len1) n
+      then T
+    else isSubstring_aux s1 s2 len1 max (n + 1)` 
+(wf_rel_tac `measure (\(s1, s2, len1, max, n). max - n)`);
+
+val isSubstring_def = Define`
+  isSubstring s1 s2 = isSubstring_aux s1 s2 (strlen s1) ((strlen s2) - (strlen s1)) 0`;
+
+(* what is going on with is string there *) 
+val result = translate isStringThere_aux_def;
+ 
+(*--------------------------------------------------------------------------------*)
+
+val compare_aux_def = tDefine "compare_aux"`
+  compare_aux (s1 : mlstring) s2 max ord n = 
+    if max <= n
+      then ord
+    else if (sub s1 n) > (sub s2 n) 
+      then GREATER
+    else if (sub s1 n) < (sub s2 n)
+      then LESS
+    else compare_aux s1 s2 max ord (n + 1)` 
+(wf_rel_tac `measure (\(s1, s2, max, ord, n). max - n)`);
+
+val compare_def = Define`
+  compare_def s1 s2 = if (strlen s1) < (strlen s2)
+    then compare_aux s1 s2 (strlen s1) GREATER 0
+  else if (strlen s2) < (strlen s1)
+    then compare_aux s1 s2 (strlen s2) LESS 0
+  else compare_aux s1 s2 (strlen s2) EQUAL 0`; 
+
+(*Pre conditions from sub *)
+val result = translate compare_aux_def;
+val result = translate compare_def;
+
+(*--------------------------------------------------------------------------------*)
+
+val collate_aux_def = tDefine "collate_aux"`
+  collate_aux f (s1 : mlstring) s2 max ord n = 
+    if max <= n 
+      then ord
+    else if f (sub s1 n) (sub s2 n) = EQUAL
+      then collate_aux f s1 s2 max ord (n + 1)
+    else
+      f (sub s1 n) (sub s2 n)`
+(wf_rel_tac `measure (\(f, s1, s2, max, ord, n). max - n)`);
+
+val collate_def = Define`
+  collate f s1 s2 = 
+  if (strlen s1) < (strlen s2)
+    then collate_aux f s1 s2 (strlen s1) GREATER 0
+  else if (strlen s2) < (strlen s1)
+    then collate_aux f s1 s2 (strlen s2) LESS 0
+  else collate_aux f s1 s2 (strlen s2) EQUAL 0`;
+
+(*Pre conditions from sub *) 
+val result = translate collate_aux_def;
+val result = translate collate_def;
+
+(*--------------------------------------------------------------------------------*)
+
+
+
 val _ = ml_prog_update (close_module NONE);
+
+(*end new stuff *)
+
+(*################################################################################*)
+
 
 
 (* CharIO -- CF verified *)
