basis/listProgScript.sml
@@ -1,0 +1,139 @@
+open preamble ml_translatorLib ml_progLib
+open listTheory
+
+(*this library depends on nothing*)
+val _ = new_theory"listProg"
+val _ = ml_prog_update (open_module "List");
+
+
+
+val _ = append_dec ``Dtabbrev ["'a"] "list" (Tapp [Tvar "'a"] (TC_name (Short "list")))``;
+
+
+val result = translate NULL_DEF;
+
+
+val result = translate LENGTH;
+
+
+val result = translate APPEND;
+
+
+val result = translate HD;
+
+val result = translate tl_def;
+val result = next_ml_names := ["tl_hol_def"];
+val result = translate TL;
+
+
+val result = translate LAST_DEF;
+
+
+val result = translate getItem_def;
+
+
+val result = translate (EL |> REWRITE_RULE[GSYM nth_def]);
+
+
+val result = translate (TAKE_def |> REWRITE_RULE[GSYM take_def]);
+
+
+val result = translate (DROP_def |> REWRITE_RULE[GSYM drop_def]);
+
+
+val result = next_ml_names := ["rev_def"];
+val result = translate REVERSE_DEF;
+
+
+val result = next_ml_names := ["concat_def"];
+val result = translate FLAT;
+
+
+val result = translate REV_DEF;
+
+
+val result = translate MAP;
+
+
+val result = translate mapPartial_def;
+
+
+val result = translate find_def;
+
+
+val result = translate FILTER;
+
+
+val result = translate partition_aux_def;
+val result = translate partition_def;
+
+
+val result = translate FOLDL;
+
+
+val result = translate FOLDR;
+
+
+val result = translate EXISTS_DEF;
+
+
+val result = next_ml_names := ["all_def"];
+val result = translate EVERY_DEF;
+
+
+val result = translate GENLIST_AUX;
+val result = translate GENLIST_GENLIST_AUX;
+val result = translate (GENLIST |> REWRITE_RULE[GSYM tabulate_def]);
+
+
+val result = translate collate_def;
+
+val result = translate zip_def;
+
+val result = translate scanl_def;
+
+val result = translate scanr_def;
+
+
+
+(*Extra translations from std_preludeLib.sml *)
+
+val result = translate SUM;
+val result = translate UNZIP;
+val result = translate SNOC;
+val result = translate PAD_RIGHT;
+val result = translate PAD_LEFT;
+val result = translate MEMBER_def;
+val result = translate (ALL_DISTAINCE |> REWRITE_RULE [MEMBER_INTRO]);
+val result = translate isPREFIX;
+val result = translate FRONT_DEF;
+val result = translate (splitAtPki_def |> REWRITE_RULE [SUC_LEMMA])
+
+val front_side_def = Q.prove(
+  `!xs. front_side xs = ~(xs = [])`,
+  Induct THEN ONCE_REWRITE_TAC [fetch "-" "front_side_def"]
+  THEN FULL_SIMP_TAC (srw_ss()) [CONTAINER_def])
+  |> update_precondition;
+
+val zip_side_def = Q.prove(
+  `!x. zip_side x = (LENGTH (FST x) = LENGTH (SND x))`,
+  Cases THEN Q.SPEC_TAC (`r`,`r`) THEN Induct_on `q` THEN Cases_on `r`
+  THEN ONCE_REWRITE_TAC [fetch "-" "zip_side_def"]
+  THEN FULL_SIMP_TAC (srw_ss()) [])
+  |> update_precondition;
+
+val el_side_def = Q.prove(
+  `!n xs. el_side n xs = (n < LENGTH xs)`,
+  Induct THEN Cases_on `xs` THEN ONCE_REWRITE_TAC [fetch "-" "el_side_def"]
+  THEN FULL_SIMP_TAC (srw_ss()) [CONTAINER_def])
+  |> update_precondition;
+
+val last_side_def = Q.prove(
+  `!xs. last_side xs = ~(xs = [])`,
+  Induct THEN ONCE_REWRITE_TAC [fetch "-" "last_side_def"]
+  THEN FULL_SIMP_TAC (srw_ss()) [CONTAINER_def])
+  |> update_precondition;
+
+
+val ml_prog_update (close_module NONE);
+val _ = export_theory()
