basis/listScript.sml
@@ -1,0 +1,158 @@
+open preamble
+
+val _ = new_theory"list"
+
+(*Data type line *)
+
+
+val tl_def = Define`
+  tl l = case l of
+    [] => [] 
+    | (h::t) => t`;
+
+
+val getItem_def = Define`
+  getItem l = case l of
+    [] => NONE
+    | (h::t) => SOME(h, t)`;
+
+
+val nth_def = Define`
+  nth l i = EL i l`;
+
+
+val take_def = Define`
+  take l i = TAKE i l`;
+
+
+
+val drop_def = Define`
+  drop l i = DROP i l`;
+
+
+val mapPartial_def = Define`
+  mapPartial f l = case l of
+    [] => []
+    | (h::t) => case (f h) of
+      NONE => mapPartial f t
+      | (SOME x) => x::(mapPartial f t)`;
+
+val mapPartial_thm = Q.store_thm (
+  "mapPartial_thm",
+  `!f l. mapPartial f l = MAP THE (FILTER IS_SOME (MAP f l))`,
+  Induct_on `l` THEN1
+  rw [mapPartial_def] \\
+  rw [mapPartial_def] \\
+  Cases_on `f h` THEN1
+    fs [IS_SOME_DEF]\\
+    rw [THE_DEF] \\
+  Cases_on `f h` THEN1
+    rw [] \\
+    fs [IS_SOME_DEF]
+)
+
+
+
+val find_def = Define`
+  find f l = case l of
+    [] => NONE
+    | (h::t) => if f h then SOME(h)
+      else find f t`;
+
+val index_find_thm = Q.prove (
+  `!x y. OPTION_MAP SND (INDEX_FIND x f l) = OPTION_MAP SND (INDEX_FIND y f l)`,
+  Induct_on `l` THEN1
+  rw [INDEX_FIND_def] \\
+  Cases_on `f h` \\
+  EVAL_TAC \\
+  rw [] \\
+  EVAL_TAC \\
+  rw []
+);
+
+
+val find_thm = Q.store_thm (
+  "find_thm",
+  `!f l. find f l = FIND f l`,
+  Induct_on `l` \\
+  rw [find_def, FIND_def, INDEX_FIND_def] \\
+  rw [find_def, FIND_def] \\
+  rw [INDEX_FIND_def] \\
+  EVAL_TAC \\
+  rw [index_find_thm]
+)
+
+
+
+
+
+val partition_aux_def = Define`
+  partition_aux f l (pos, neg) = case l of
+    [] => (REVERSE pos, REVERSE neg)
+    | (h::t) => if f h then partition_aux f t ((h::pos), neg)
+      else partition_aux f t (pos, (h::neg))`;
+
+val partition_aux_thm = Q.prove(
+  `!f l l1 l2. partition_aux f l l1 l2 = (REVERSE l1++(FILTER f l), REVERSE l2++(FILTER ($~ o f) l))`,
+  Induct_on `l` \\
+  rw [partition_aux_def] \\
+  rw [partition_aux_def]
+); 
+
+val partition_pos_thm = Q.store_thm(
+  "partition_pos_thm",
+  `!f l. FST (partition f l) = FILTER f l`,
+  rw [partition_def, FILTER, partition_aux_thm]
+);
+
+val partition_neg_thm = Q.store_thm(
+  "partition_neg_thm",
+  `!f l. SND (partition f l) = FILTER ($~ o f) l`,
+  rw [partition_def, FILTER, partition_aux_thm]
+);
+
+
+
+val tabulate_def = Define`
+  tabulate n f = GENLIST f n`;
+
+
+val collate_def = Define`
+  (collate f [] [] = EQUAL) /\
+  (collate f [] (h::t) = LESS) /\
+  (collate f (h::t) [] = GREATER) /\
+  (collate f (h1::t1) (h2::t2) =
+    if f h1 h2 = EQUAL
+      then collate f t1 t2
+    else f h1 h2)`;
+
+val collate_equal_thm = Q.store_thm (
+  "collate_equal_thm",
+  `!l. (!x. MEM x l ==> f x x = EQUAL) ==> collate f l l = EQUAL`,
+  Induct_on `l` \\
+  rw [collate_def] \\
+  rw [collate_def]
+);
+
+
+val zip_def = Define`
+  (zip [] [] = []) /\
+  (zip [] (h::t) = []) /\
+  (zip (h::t) [] = []) /\
+  (zip (h1::t1) (h2::t2) = (h1, h2)::(zip t1 t2))`;
+
+
+(* from std_preludeLib *)
+val LENGTH_AUX_def = Define `
+  (LENGTH_AUX [] n = (n:num)) /\
+  (LENGTH_AUX (x::xs) n = LENGTH_AUX xs (n+1))`;
+
+val LENGTH_AUX_THM = Q.prove(
+  `!xs n. LENGTH_AUX xs n = LENGTH xs + n`,
+  Induct THEN ASM_SIMP_TAC std_ss [LENGTH_AUX_def,LENGTH,ADD1,AC ADD_COMM ADD_ASSOC])
+  |> Q.SPECL [`xs`,`0`] |> GSYM |> SIMP_RULE std_ss [];
+
+val SUC_LEMMA = Q.prove(`SUC = \x. x+1`,SIMP_TAC std_ss [FUN_EQ_THM,ADD1]);
+
+
+val _ = export_theory()
