basis/mlstringProgScript.sml
@@ -1,0 +1,68 @@
+open preamble 
+  ml_translatorLib ml_progLib
+open mlstringTheory
+
+val _ = new_theory"mlstringProg"
+
+val _ = translation_extends "listProg";
+
+val _ = ml_prog_update (open_module "String");
+
+val res = append_dec ``Dlet (Pvar "size") (Fun "x" (App (Strlen) [Var(Short"x")]))``;
+val _ = trans "explode" `explode`
+val _ = trans "implode" `implode`
+val _ = trans "size" `strlen`
+
+
+val result = translate EL;
+val result = translate sub_def;
+
+
+val result = translate extract_aux_def;
+val result = translate extract_def;
+val result = translate substring_def;
+
+
+val result = translate strcat_def;
+
+val result = translate stringListToChars_def;
+val result = translate concat_def;
+
+val result = translate concatWith_aux_def;
+val result = translate concatWith_def;
+
+val result = translate str_def;
+
+translate explode_aux_def;
+translate explode_def;
+
+val result = translate translate_aux_def;
+val result = translate translate_def;
+
+(*these have pre-conditions because sub has a precondition *)
+val result = translate tokens_aux_def;
+val result = translate tokens_def;
+
+val result = translate fields_aux_def;
+val result = translate fields_def;
+
+(*These may also not be translating because of the sub precondition *)
+val result = translate isStringThere_aux_def;
+val result = translate isPrefix_def;
+val result = translate isSuffix_def;
+val result = translate is Substring_aux;
+
+(*Pre conditions from sub *)
+val result = translate compare_aux_def;
+val result = translate compare_def;
+
+
+(*Pre conditions from sub *)
+val result = translate collate_aux_def;
+val result = translate collate_def;
+
+
+val _ = ml_prog_update (close_module NONE);
+
+val _ = export_theory()
+
