basis/mlstringScript.sml
@@ -1,0 +1,356 @@
+(*
+   Small theory of wrapped strings, so the translator can distinguish
+   them from char lists and can target CakeML strings directly.
+*)
+open preamble
+
+val _ = new_theory"mlstring"
+
+(* TODO: move *)
+val irreflexive_inv_image = Q.store_thm("irreflexive_inv_image",
+  `!R f. irreflexive R ==> irreflexive (inv_image R f)`,
+  SIMP_TAC std_ss [irreflexive_def,inv_image_def])
+
+val trichotomous_inv_image = Q.store_thm("trichotomous_inv_image",
+  `!R f. trichotomous R /\ (INJ f UNIV UNIV) ==> trichotomous (inv_image R f)`,
+  SIMP_TAC std_ss [trichotomous,inv_image_def,INJ_DEF,IN_UNIV] THEN
+  METIS_TAC[])
+
+(* Defines strings as a separate type from char list. This theory should be
+   moved into HOL, either as its own theory, or as an addendum to stringTheory *)
+
+val _ = Datatype`mlstring = strlit string`
+
+(*
+It should be like this when the primitives change in CakeML:
+
+(* assume these are primitive... *)
+val length_def = Define`
+  length (strlit s) = LENGTH s`;
+val sub_def = Define`
+  sub (strlit s) n = EL n s`;
+val implode_def = Define`
+  implode = strlit`
+
+val explode_aux_def = Define`
+  explode_aux s n = if n < length s then sub s n :: (explode_aux s (n+1)) else []`;
+val explode_def = Define`
+  explode s = explode_aux s 0`;
+val explode_aux_thm = Q.prove(
+  `explode_aux (strlit s) n = DROP n s`,
+
+val explode_thm = Q.store_thm("explode_thm",
+  `explode (strlit s) = s`,
+  ...);
+*)
+
+val implode_def = Define`
+  implode = strlit`
+
+val explode_def = Define`
+  explode (strlit ls) = ls`
+val _ = export_rewrites["explode_def"]
+
+val explode_implode = Q.store_thm("explode_implode",
+  `∀x. explode (implode x) = x`,
+  rw[implode_def])
+
+val implode_explode = Q.store_thm("implode_explode",
+  `∀x. implode (explode x) = x`,
+  Cases >> rw[implode_def])
+
+val explode_11 = Q.store_thm("explode_11",
+  `∀s1 s2. explode s1 = explode s2 ⇔ s1 = s2`,
+  Cases >> Cases >> simp[])
+
+val implode_BIJ = Q.store_thm("implode_BIJ",
+  `BIJ implode UNIV UNIV`,
+  rw[BIJ_IFF_INV] >>
+  qexists_tac`explode` >>
+  rw[implode_explode,
+     explode_implode])
+
+val explode_BIJ = Q.store_thm("explode_BIJ",
+  `BIJ explode UNIV UNIV`,
+  rw[BIJ_IFF_INV] >>
+  qexists_tac`implode` >>
+  rw[implode_explode,
+     explode_implode])
+
+val strlen_def = Define`
+  strlen s = LENGTH (explode s)`;
+
+val sub_def = Define`
+  sub s n =  EL n (explode s)`;
+
+(* TODO: write a bunch of string functions in terms of strlen and sub *)
+(* TODO: strlen should be called size ? or length ? *)
+
+
+val extract_aux_def = tDefine "extract_aux"`
+    extract_aux s n max =
+    if max <= n
+      then []
+    else (sub s n)::(extract_aux s (n + 1) max)`
+(wf_rel_tac `measure (\(s, n, max). max - n)`)
+
+
+val extract_def = Define`
+  extract s i opt = case opt of
+    (SOME x) => implode (extract_aux s i (THE opt))
+    | NONE => implode (extract_aux s i (strlen s))`;
+
+val substring_def = Define`
+  substring s i j = implode (extract_aux s i j)`;
+
+
+(* TODO: don't explode/implode once CakeML supports string append *)
+val strcat_def = Define`
+  strcat s1 s2 = implode(explode s1 ++ explode s2)`
+val _ = Parse.add_infix("^",480,Parse.LEFT)
+val _ = Parse.overload_on("^",``λx y. strcat x y``)
+
+val stringListToChars_def = Define`
+  stringListToChars l = case l of 
+    [] => []
+    | ([]::t) => stringListToChars t
+    | ((hh::ht)::t) => hh::stringListToChars(ht::t)`;
+
+val concat_def = Define`
+  concat l = implode (stringListToChars l)`;
+
+(*NEED TO PROVE TERMINATION*)
+(*may be a bit complex to attempt to save memory (passing around a lot)*)
+val concatWith_aux_def = Define`
+  concatWith_aux l s ss bool =
+  if bool then
+    case l of
+      [] => []
+      | []::[] => []
+      | ([]::t) => concatWith_aux t s s F
+      | ((hh::ht)::t) => hh::(concatWith_aux (ht::t) s ss T)
+  else
+    case ss of
+      [] => concatWith_aux l s ss T
+      | (h::t) => h::(concatWith_aux l s t F) `;
+
+val concatWith_def = Define`
+    concatWith s l = implode (concatWith_aux l s s T)`;
+
+val str_def = Define`
+  str (c: char) = [c]`;
+
+val explode_aux_def = tDefine "explode_aux"`
+  explode_aux s max n =
+    if max <= n then []
+    else (sub s n)::(explode_aux s max (n + 1))`
+(wf_rel_tac `measure (\(s, max, n). max - n)`);
+
+val explode_def = Define`
+  explode s = explode_aux s (strlen s) 0`;
+
+val translate_aux_def = tDefine "translate_aux"`
+  translate_aux f s max n = 
+    if max <= n then []
+    else f (sub s n)::(translate_aux f s max (n + 1))`
+(wf_rel_tac `measure (\(f, s, max, n). max - n)`);
+
+
+val translate_def = Define`
+  translate f s = implode (translate_aux f s (strlen s) 0)`;
+(*TODO: Check the functionality *)
+val tokens_aux_def = tDefine "tokens_aux"`
+  tokens_aux f s ss max n =
+  if max <= n
+    then []
+  else if (f (sub s n) /\ ~(ss = []))
+    then ss::(tokens_aux f s [] max (n + 1))
+  else if f (sub s n)
+    then tokens_aux f s ss max (n + 1)
+  else tokens_aux f s ((sub s n)::ss) max (n + 1)`
+(wf_rel_tac `measure (\(f, s, ss, max, n). max - n)`);
+
+
+
+val tokens_def = Define `
+  tokens f s = tokens_aux f s [] (strlen s) 0`;
+
+fun tokens_aux (f : char -> bool) s ss max n =
+  if max <= n
+    then []
+  else if (f (String.sub s n)) andalso not(ss = [])
+    then ss::(tokens_aux f s [] max (n + 1))
+  else if f (String.sub s n)
+    then tokens_aux f s ss max (n + 1)
+  else tokens_aux f s ((String.sub s n)::ss) max (n + 1)
+
+
+(*TODO: Check the functionality *)
+val fields_aux_def = tDefine "fields_aux"`
+  fields_aux f s ss max n =
+  if max <= n
+    then []
+  else if f (sub s n)
+    then ss::(fields_aux f s [] max (n + 1))
+  else fields_aux f s ((sub s n)::ss) max (n + 1)`
+(wf_rel_tac `measure (\(f, s, ss, max, n). max - n)`);
+
+val fields_def = Define`
+  fields f s = fields_aux f s [] (strlen s) 0`;
+
+
+
+(*this could be one less iteration if the check is for n + 1 *)
+val isStringThere_aux_def = tDefine "isPrefix_aux"`
+  isStringThere_aux s1 s2 max n =
+  if max <= n
+    then T
+  else if (sub s1 n) = (sub s2 n)
+    then isStringThere_aux s1 s2 max (n + 1)
+  else F`
+(wf_rel_tac `measure (\(s1, s2, max, n). max - n)`);
+
+val isPrefix_def = Define`
+  isPrefix s1 s2 = isStringThere_aux s1 s2 (strlen s1) 0`;
+
+val isSuffix_def = Define`
+  isSuffix s1 s2 = isStringThere_aux s1 s2 (strlen s2) ((strlen s2) - (strlen s1))`;
+
+val isSubstring_aux_def = tDefine "isSubstring_aux"`
+  isSubstring_aux s1 s2 len1 max n =
+    if max <= n
+      then F
+    else if isStringThere_aux s1 s2 (n + len1) n
+      then T
+    else isSubstring_aux s1 s2 len1 max (n + 1)`
+(wf_rel_tac `measure (\(s1, s2, len1, max, n). max - n)`);
+
+val isSubstring_def = Define`
+  isSubstring s1 s2 = isSubstring_aux s1 s2 (strlen s1) ((strlen s2) - (strlen s1)) 0`;
+
+
+
+val compare_aux_def = tDefine "compare_aux"`
+  compare_aux (s1 : mlstring) s2 max ord n =
+    if max <= n
+      then ord
+    else if (sub s1 n) > (sub s2 n)
+      then GREATER
+    else if (sub s1 n) < (sub s2 n)
+      then LESS
+    else compare_aux s1 s2 max ord (n + 1)`
+(wf_rel_tac `measure (\(s1, s2, max, ord, n). max - n)`);
+
+val compare_def = Define`
+  compare_def s1 s2 = if (strlen s1) < (strlen s2)
+    then compare_aux s1 s2 (strlen s1) GREATER 0
+  else if (strlen s2) < (strlen s1)
+    then compare_aux s1 s2 (strlen s2) LESS 0
+  else compare_aux s1 s2 (strlen s2) EQUAL 0`;
+
+
+
+val collate_aux_def = tDefine "collate_aux"`
+  collate_aux f (s1 : mlstring) s2 max ord n =
+    if max <= n
+      then ord
+    else if f (sub s1 n) (sub s2 n) = EQUAL
+      then collate_aux f s1 s2 max ord (n + 1)
+    else
+      f (sub s1 n) (sub s2 n)`
+(wf_rel_tac `measure (\(f, s1, s2, max, ord, n). max - n)`);
+
+val collate_def = Define`
+  collate f s1 s2 =
+  if (strlen s1) < (strlen s2)
+    then collate_aux f s1 s2 (strlen s1) GREATER 0
+  else if (strlen s2) < (strlen s1)
+    then collate_aux f s1 s2 (strlen s2) LESS 0
+  else collate_aux f s1 s2 (strlen s2) EQUAL 0`;
+
+
+
+
+
+
+
+
+
+
+
+
+
+
+
+
+
+
+
+
+
+
+
+
+
+
+
+
+
+
+val mlstring_lt_def = Define`
+  mlstring_lt (strlit s1) (strlit s2) ⇔
+    string_lt s1 s2`
+
+val mlstring_lt_inv_image = Q.store_thm("mlstring_lt_inv_image",
+  `mlstring_lt = inv_image string_lt explode`,
+  simp[inv_image_def,FUN_EQ_THM] >>
+  Cases >> Cases >> simp[mlstring_lt_def])
+
+val transitive_mlstring_lt = Q.prove(
+  `transitive mlstring_lt`,
+  simp[mlstring_lt_inv_image] >>
+  match_mp_tac transitive_inv_image >>
+  metis_tac[transitive_def,string_lt_trans])
+
+val irreflexive_mlstring_lt = Q.prove(
+  `irreflexive mlstring_lt`,
+  simp[mlstring_lt_inv_image] >>
+  match_mp_tac irreflexive_inv_image >>
+  simp[irreflexive_def,string_lt_nonrefl])
+
+val trichotomous_mlstring_lt = Q.prove(
+  `trichotomous mlstring_lt`,
+  simp[mlstring_lt_inv_image] >>
+  match_mp_tac trichotomous_inv_image >>
+  reverse conj_tac >- metis_tac[explode_BIJ,BIJ_DEF] >>
+  metis_tac[trichotomous,string_lt_cases])
+
+val StrongLinearOrder_mlstring_lt = Q.store_thm("StrongLinearOrder_mlstring_lt",
+  `StrongLinearOrder mlstring_lt`,
+  rw[StrongLinearOrder,trichotomous_mlstring_lt,
+     StrongOrder,irreflexive_mlstring_lt,transitive_mlstring_lt])
+
+val mlstring_cmp_def = Define`
+  mlstring_cmp = TO_of_LinearOrder mlstring_lt`
+
+val TotOrd_mlstring_cmp = Q.store_thm("TotOrd_mlstring_cmp",
+  `TotOrd mlstring_cmp`,
+  simp[mlstring_cmp_def] >>
+  match_mp_tac TotOrd_TO_of_Strong >>
+  simp[StrongLinearOrder_mlstring_lt])
+
+val ALL_DISTINCT_MAP_implode = Q.store_thm("ALL_DISTINCT_MAP_implode",
+  `ALL_DISTINCT ls ⇒ ALL_DISTINCT (MAP implode ls)`,
+  strip_tac >>
+  match_mp_tac ALL_DISTINCT_MAP_INJ >>
+  rw[implode_def])
+val _ = export_rewrites["ALL_DISTINCT_MAP_implode"]
+
+val ALL_DISTINCT_MAP_explode = Q.store_thm("ALL_DISTINCT_MAP_explode",
+  `∀ls. ALL_DISTINCT (MAP explode ls) ⇔ ALL_DISTINCT ls`,
+  gen_tac >> EQ_TAC >- MATCH_ACCEPT_TAC ALL_DISTINCT_MAP >>
+  STRIP_TAC >> MATCH_MP_TAC ALL_DISTINCT_MAP_INJ >>
+  simp[explode_11])
+val _ = export_rewrites["ALL_DISTINCT_MAP_explode"]
+
+val _ = export_theory()
