basis/optionProgScript.sml
@@ -1,0 +1,57 @@
+open preamble ml_translatorLib ml_progLib
+open optionTheory
+
+(*this library depends on nothing *)
+val _ = new_theory"optionProg"
+val _ = ml_prog_update (open_module "Option");
+
+val _ = append_dec ``Dtabbrev ["'a"] "option" (Tapp [Tvar "'a"] (TC_name (Short "option")))``;
+
+val result = translate IS_SOME_DEF;
+
+val result = translate getOpt_def;
+
+val result = translate IS_SOME_DEF;
+
+val result = next_ml_names := ["valOf_def"];
+val result = translate THE_DEF;
+
+val result = next_ml_names := ["join_def"];
+val result = translate OPTION_JOIN_DEF;
+
+val result = next_ml_names := ["map_def"];
+val result = translate OPTION_MAP_DEF;
+
+val result = translate (OPTION_BIND_def |> REWRITE_RULE[GSYM mapPartial_def]);
+
+val result = translate compose_def;
+
+val result = translate composePartial_def;
+
+(*Functions declared in std_preludeLib *)
+val result = translate IS_NONE_DEF;
+val result = translate IS_OPTION_MAP2_DEF;
+
+val res = translate THE_DEF;
+val res = translate IS_NONE_DEF;
+val res = translate IS_SOME_DEF;
+val res = translate OPTION_MAP_DEF;
+val res = translate OPTION_MAP2_DEF;
+
+val the_side_def = Q.prove(
+  `the_side = IS_SOME`,
+  FULL_SIMP_TAC std_ss [FUN_EQ_THM] THEN Cases
+  THEN FULL_SIMP_TAC (srw_ss()) [fetch "-" "the_side_def"])
+  |> update_precondition;
+
+val option_map2_side_def = Q.prove(
+  `!f x y. option_map2_side f x y = T`,
+  FULL_SIMP_TAC (srw_ss()) [fetch "-" "option_map2_side_def",the_side_def])
+  |> update_precondition;
+
+
+
+
+val ml_prog_update (close_module NONE);
+val _ = export_theory() 
+
