basis/optionScript.sml
@@ -1,0 +1,28 @@
+open preamble 
+
+val _ = new_theory"option"
+
+(*val _ = Datatype `option = *)
+
+
+val getOpt_def = Define`
+  getOpt opt a = case opt of
+    (SOME v) => v
+    | NONE => a`;
+
+val filter_def  = Define`
+  filter f a = if f a then SOME(a) else NONE`;
+
+val compose_def = Define`
+  compose f g a = case g a of
+    (SOME v) => SOME(f v)
+    | NONE => NONE`;
+
+val composePartial_def = Define`
+  composePartial f g a = case g a of
+    (SOME v) => f v
+    | NONE => NONE`;
+
+
+
+val _ = export_theory() 
